close fairness sketch

theories/playground/pure_threadpool_sim.v
@@ -24,13 +24,17 @@ Section fair_termination_preservation.
 
   (* an expression is active in a thread pool,
      if it is not a value *)
-  Definition active_exprs T :=
+  Definition active_threads T :=
     list_to_set (C := gset nat) (fmap fst (filter (λ '(i, e), ¬ val e) (imap pair T))).
 
-  Lemma active_expr_spec T i:
-    i ∈ active_exprs T ↔ ∃ e, T !! i = Some e ∧ ¬ val e.
+  Definition threads T :=
+    list_to_set (C := gset nat) (seq 0 (length T)).
+
+
+  Lemma active_threads_spec T i:
+    i ∈ active_threads T ↔ ∃ e, T !! i = Some e ∧ ¬ val e.
   Proof.
-    rewrite /active_exprs elem_of_list_to_set elem_of_list_fmap.
+    rewrite /active_threads elem_of_list_to_set elem_of_list_fmap.
     split.
     - intros [[i' e] [-> Hlook]]; simpl.
       eapply elem_of_list_filter in Hlook as [? Hlook].
@@ -42,37 +46,31 @@ Section fair_termination_preservation.
       eexists _, _. split; done.
   Qed.
 
-
-  Lemma active_exprs_remove P i e O:
-    (O ⊆ active_exprs P.(tgt)) →
-    (O ∖ {[i]} ⊆ active_exprs (<[i:=e]> P.(tgt))).
-  Proof using val_no_step.
-  intros Hsub j Hel. eapply elem_of_difference in Hel as [Hj Hne].
-  assert (j ≠ i) as Hne' by set_solver.
-  eapply active_expr_spec.
-  eapply Hsub in Hj. eapply active_expr_spec in Hj as (e' & Hlook & Hnval).
-  exists e'. rewrite list_lookup_insert_ne; last done. split; done.
+  Lemma threads_spec T i:
+    i ∈ threads T ↔ ∃ e, T !! i = Some e.
+  Proof.
+    rewrite /active_threads elem_of_list_to_set elem_of_seq.
+    split.
+    - intros [_ Hlt]. eapply lookup_lt_is_Some_2. lia.
+    - intros ? % lookup_lt_is_Some_1. lia.
   Qed.
 
-  Lemma active_exprs_update T i e O:
-    (O ⊆ active_exprs T) →
-    ¬ val e →
-    O ⊆ active_exprs (<[i:=e]> T).
+  Lemma threads_update T i e:
+    threads T ⊆ threads (<[i:=e]> T).
   Proof using val_no_step.
-  intros Hsub Hnval j Hel.
-  eapply active_expr_spec.
-  eapply Hsub in Hel. eapply active_expr_spec in Hel as (e' & Hlook & Hnval').
-  destruct (decide (i = j)).
-  - subst; exists e. split; last done.
-    eapply list_lookup_insert, lookup_lt_Some, Hlook.
-  - rewrite list_lookup_insert_ne; last done. exists e'. split; done.
+    intros j [e' Hlook]%threads_spec.
+    eapply threads_spec.
+    destruct (decide (i = j)).
+    - subst; exists e.
+      eapply list_lookup_insert, lookup_lt_Some, Hlook.
+    - rewrite list_lookup_insert_ne; last done. by exists e'.
   Qed.
 
-  Lemma active_exprs_weaken T T':
-    active_exprs T ⊆ active_exprs (T ++ T').
+  Lemma threads_weaken T T':
+    threads T ⊆ threads (T ++ T').
   Proof using val_no_step.
-    intros j (e & Hlook & Hnval)%active_expr_spec.
-    eapply active_expr_spec. exists e. split; last done.
+    intros j (e & Hlook)%threads_spec.
+    eapply threads_spec. exists e.
     eapply lookup_app_l_Some, Hlook.
   Qed.
 
@@ -105,7 +103,7 @@ Section fair_termination_preservation.
     fair_pool_step T D i T' D'.
 
   Definition delays_for T D :=
-    ∀ i, i ∈ active_exprs T → is_Some (D !! i).
+    ∀ i, i ∈ active_threads T → is_Some (D !! i).
 
 
 
@@ -129,6 +127,14 @@ Section fair_termination_preservation.
       rewrite insert_app_r. simpl.
       rewrite -app_assoc; simpl.
       econstructor; auto.
+  Qed.
+
+  Lemma pool_steps_single T i T':
+    pool_step T i T' →
+    pool_steps T {[i]} T'.
+  Proof using val_no_step.
+    intros Hstep; econstructor; [eauto|constructor|].
+    set_solver.
   Qed.
 
   Lemma pool_step_value_preservation e T i j T':
@@ -159,7 +165,7 @@ Section fair_termination_preservation.
       ∃ e e' T_f, step e e' T_f ∧
       T !! i = Some e ∧
       T' = <[i := e']> T ++ T_f ∧
-      D !! i = Some 0 ∧
+      (* D !! i = Some 0 ∧ *)
       (∀ j n, j ≠ i → D !! j = Some n → ∃ n', n = S n' ∧ D' !! j = Some n').
   Proof.
     destruct 1 as [i T T' D D' Pool HD Hdecr].
@@ -188,14 +194,14 @@ Section fair_termination_preservation.
     (∃ e_s', step e_s e_s' ∧ least e_t e_s') ∨ *)
     (* target step case *)
     ((∃ e_t' T_t, step e_t e_t' T_t) ∧
+     (∀ e_t' T_t, step e_t e_t' T_t →
       (* stuttering *)
-      ((∀ e_t' efs, step e_t e_t' efs → efs = [] ∧ inner e_t' e_s) ∨
+      (T_t = [] ∧ inner e_t' e_s) ∨
       (* no stuttering *)
-      (∀ e_t' T_t, step e_t e_t' T_t →
-      ∃ e_s' T_s, step e_s e_s' T_s ∧
-      length T_t = length T_s ∧
-        ∀ e_t e_s, (e_t, e_s) ∈ zip (e_t' :: T_t) (e_s' :: T_s) → outer e_t e_s
-    ))).
+      (∃ e_s' T_s, step e_s e_s' T_s ∧
+        length T_t = length T_s ∧
+        ∀ e_t e_s, (e_t, e_s) ∈ zip (e_t' :: T_t) (e_s' :: T_s) → outer e_t e_s)
+    )).
 
   Definition sim_expr_body outer := lfp (sim_expr_inner outer).
   Definition sim_expr := gfp sim_expr_body.
@@ -238,8 +244,8 @@ Section fair_termination_preservation.
   Proof using val_no_step is_val.
     rewrite sim_expr_unfold sim_expr_body_unfold /sim_expr_inner.
     intros [[Ht Hs]|Hstep] Htgt; first (exfalso; eapply val_no_step; [apply Ht|]; eauto).
-    destruct Hstep as [_ [Hstep|Hstep]].
-    - left. edestruct Hstep; eauto. split; first done.
+    destruct Hstep as [_ Hstep]. destruct (Hstep _ _ Htgt) as [[-> Hsim]|].
+    - left. split; first done.
       by rewrite sim_expr_unfold. (* todo: include this in the unfold *)
     - right. eauto.
   Qed.
@@ -247,9 +253,12 @@ Section fair_termination_preservation.
   (* Thread Pool Simulation *)
 
   (* we define the pool simulation *)
+  Definition all_values (O: gset nat) P :=
+    (∀ i e_t e_s, i ∈ O → P !! i = Some (e_t, e_s) → val e_t ∧ val e_s).
+
   Definition must_step (post: pool → Prop) (must_step: pool → gset nat → list nat → Prop) (P: pool) (O: gset nat) (D: delays) :=
-    delays_for (P.(tgt)) D →
-    ((∀ i, i ∈ O → ∃ e_t e_s, P !! i = Some (e_t, e_s) ∧ val e_t ∧ val e_s) ∧ post P) ∨
+    delays_for P.(tgt) D →
+    (all_values O P ∧ post P) ∨
     ((∃ T_t' i, pool_step P.(tgt) i T_t') ∧
      (∀ T_t' D' i,
         fair_pool_step P.(tgt) D i T_t' D' →
@@ -259,8 +268,7 @@ Section fair_termination_preservation.
   )).
 
   Definition sim_pool_body (sim_pool: pool → Prop) (P: pool) :=
-    (∀ e_t e_s, (e_t, e_s) ∈ P → val e_t → val e_s) ∧
-    ∀ D O, O ⊆ active_exprs P.(tgt) → lfp (must_step sim_pool) P O D.
+    ∀ D, lfp (must_step sim_pool) P (threads P.(tgt)) D.
 
   Definition sim_pool := gfp sim_pool_body.
 
@@ -296,11 +304,7 @@ Section fair_termination_preservation.
 *)
 
 Definition sim_expr_all P := (∀ e_t e_s, (e_t, e_s) ∈ P → sim_expr e_t e_s).
-Definition local_all := lfp (must_step sim_expr_all).
-Definition local_steps O P :=
-  ∀ D,
-  O ⊆ active_exprs (P.*1) →
-  local_all P O D.
+Notation local_all := (lfp (must_step sim_expr_all)).
 
 
 Lemma local_all_add_values P O O' D:
@@ -310,13 +314,14 @@ Lemma local_all_add_values P O O' D:
 Proof using val_no_step.
   intros Hall; revert P O D Hall O'.
   change (local_all ⪯ λ P O D, ∀ O' : gset nat,
-    (∀ i : nat, i ∈ O' → i ∈ O ∨ (∃ e_t e_s, P !! i = Some (e_t, e_s) ∧ val e_t ∧ val e_s))
+    (∀ i : nat, i ∈ O' → i ∈ O ∨ ∃ e_t e_s, P !! i = Some (e_t, e_s) ∧ val e_t ∧ val e_s)
     → local_all P O' D).
   eapply lfp_least_pre_fixpoint; intros P O D Hsim O' Hel.
-  rewrite /local_all lfp_fixpoint {1}/must_step.
+  rewrite lfp_fixpoint {1}/must_step.
   intros Hdel. specialize (Hsim Hdel) as [Base|Step].
   - left. destruct Base as [Base ?]; split; last done.
-    intros i Hi. destruct (Hel _ Hi) as [?|]; by eauto.
+    intros i e_t e_s Hi. destruct (Hel _ Hi) as [?|(? & ? & Hlook & ? & ?)]; eauto.
+    intros Hlook'. rewrite Hlook in Hlook'. injection Hlook' as -> ->. eauto.
   - right. destruct Step as [? Step]; split; first done.
     intros T_t' D' i Hstep. destruct (Step T_t' D' i Hstep) as (P' & I & Heq & Hsteps & Hpost).
     exists P', I. split; first done. split; first done.
@@ -342,12 +347,10 @@ Proof using val_no_step.
   naive_solver.
 Qed.
 
-
-
 Lemma local_all_delay_for P O D:
   (delays_for P.(tgt) D → local_all P O D) → local_all P O D.
 Proof.
-  rewrite /local_all lfp_fixpoint.
+  rewrite lfp_fixpoint.
   rewrite /must_step; intros Hstep Hdel; eapply (Hstep Hdel Hdel).
 Qed.
 
@@ -362,148 +365,138 @@ Proof.
   - by eapply Hall, elem_of_list_lookup_2.
 Qed.
 
+Lemma sim_expr_all_app P P' :
+  sim_expr_all P → sim_expr_all P' → sim_expr_all (P ++ P').
+Proof.
+  intros HP HP' e_t e_s [|]%elem_of_app; eauto.
+Qed.
+
+
+Lemma local_all_stuttered i e_t e_t' e_s P O D' T_t':
+  T_t' = <[i := e_t']> P.(tgt) →
+  P !! i = Some (e_t, e_s) →
+  local_all (<[i := (e_t', e_s)]> P) O D' →
+  ∃ P' (I : gset nat), P'.(tgt) = T_t' ∧ pool_steps P.(src) I P'.(src) ∧ local_all P' (O ∖ I) D'.
+Proof using val_no_step.
+  intros Hupd Hlook Hall; exists (<[i := (e_t', e_s)]> P), ∅.
+  rewrite !list_fmap_insert; split; first done.
+  rewrite list_insert_id; last rewrite list_lookup_fmap Hlook //.
+  split; first constructor. eapply local_all_weaken; eauto. set_solver.
+Qed.
+
+Lemma local_all_not_stuttered i e_t e_t' e_s e_s' P O D' T_t' T_f_s T_f_t:
+  T_t' = <[i := e_t']> P.(tgt) ++ T_f_t →
+  P !! i = Some (e_t, e_s) →
+  step e_s e_s' T_f_s →
+  length T_f_t = length T_f_s →
+  local_all (<[i := (e_t', e_s')]> P ++ zip T_f_t T_f_s) (O ∖ {[i]}) D' →
+  ∃ P' (I : gset nat), P'.(tgt) = T_t' ∧ pool_steps P.(src) I P'.(src) ∧ local_all P' (O ∖ I) D'.
+Proof using val_no_step.
+  intros Hupd Hlook Hstep Hlen Hall; exists (<[i := (e_t', e_s')]> P ++ zip T_f_t T_f_s), {[i]}.
+  rewrite !fmap_app fst_zip ?Hlen // snd_zip ?Hlen // !list_fmap_insert Hupd.
+  split; first done.
+  split.
+  { eapply pool_steps_single, pool_step_iff.
+    do 3 eexists; repeat split; first done.
+    rewrite list_lookup_fmap Hlook //=. }
+  done.
+Qed.
+
+
+
 Lemma sim_expr_to_pool P:
   sim_expr_all P → sim_pool P.
-Proof.
+Proof using val_no_step.
   revert P. change (sim_expr_all ⪯ sim_pool).
-  eapply gfp_greatest_post_fixpoint. intros P Hsim. split.
-  - intros e_t e_s Hel Hval. eapply sim_expr_val; last done. eapply (Hsim e_t e_s Hel).
-  - intros D O; revert D. change (local_steps O P).
-    revert P Hsim. induction O as [O IH] using set_strong_ind.
-    destruct (decide (O ≡ ∅)) as [Empty|[i Hel]%set_choose].
-    + intros P Hsize D Hsub. rewrite /local_all lfp_fixpoint {1}/must_step.
-      intros Hdel. left. split; last done.
-      intros i; set_solver.
-    + intros P Hall D Hsub.
-      specialize (Hsub _ Hel) as Hactive.
-      eapply active_expr_spec in Hactive as (e & Hlook & Hnval).
-      eapply list_lookup_fmap_inv in Hlook as ([e_t e_s] & -> & Hlook).
-      simpl in Hnval.
-      assert (sim_expr e_t e_s) as Hsim by eapply Hall, elem_of_list_lookup_2, Hlook.
-      revert Hsim; rewrite sim_expr_unfold /sim_expr_body; intros Hsim.
-      revert e_t e_s Hsim P Hall Hnval Hlook D Hsub.
-      change (lfp (sim_expr_inner sim_expr) ⪯
-              λ e_t e_s, ∀ P,
-                sim_expr_all P →
-                ¬ val e_t →
-                P !! i = Some (e_t, e_s) →
-                local_steps O P).
-      eapply lfp_strong_ind; first apply _.
-      intros e_t e_s Hinner P Hall Hnval Hlook D Hsub.
-      destruct Hinner as [Val|[CanStep AllSteps]].
-      * naive_solver.
-      * eapply local_all_delay_for; intros Hdom.
-        destruct (Hdom i) as [d HD]; first apply Hsub, Hel.
-        clear Hdom.
-        revert D P HD Hsub Hall Hlook.
-        induction d as [|d IHd].
-        -- intros D P HD Hsub Hall Hlook.
-           rewrite /local_all lfp_fixpoint {1}/must_step.
-           intros Hdom.
-           right. split.
-           { destruct CanStep as (e' & T_f & Hstep).
-             exists (<[i := e']> P.*1 ++ T_f), i.
-             eapply pool_step_iff. do 3 eexists; split; first eauto.
-             split; last done. by rewrite list_lookup_fmap Hlook. }
-           intros T_t' D' j Hpool.
-           (* eapply fair_pool_step_inv in Hpool as (e_t_dup & e_t' & T_f & Hstep & Hdup & Hupd & Hj). *)
-           eapply fair_pool_step_zero_inv in Hpool; last done.
-           eapply (pool_step_iff) in Hpool as (e_t_dup & e_t' & T_f & Hstep & Hlook' & Hupd).
-           assert (e_t_dup = e_t) as ->; last clear Hlook'.
-           { revert Hlook'; rewrite list_lookup_fmap Hlook //=; naive_solver. }
-           destruct AllSteps as [Stutter|NoStutter].
-           ++ specialize (Stutter _ _ Hstep) as [-> Hcont].
-              exists (<[i := (e_t', e_s)]> P), ∅.
-              split. { by rewrite Hupd list_fmap_insert //= right_id. }
-              split.
-              { rewrite list_fmap_insert //= list_insert_id; first by constructor.
-                rewrite list_lookup_fmap Hlook //=. }
-              destruct (decide (val e_t')).
-              ** revert Hcont. rewrite meet_right.
-                 change (lfp (sim_expr_inner _) _ _) with (sim_expr_body sim_expr e_t' e_s).
-                 rewrite -sim_expr_unfold. intros sim.
-                 assert (val e_s) as v' by by eapply sim_expr_val.
-                 eapply (local_all_add_values _ (O ∖ {[i]})).
-                 { eapply IH.
-                   - eapply subset_difference_elem_of, Hel.
-                   - by eapply sim_expr_all_insert.
-                   - rewrite list_fmap_insert //=. by eapply active_exprs_remove.
-                 }
-                 { intros k Hk. eapply elem_of_difference in Hk as [Hk _].
-                   destruct (decide (i = k)); first subst.
-                   - right. exists e_t', e_s. repeat split; auto.
-                     eapply list_lookup_insert, lookup_lt_Some, Hlook.
-                   - left. set_solver.
-                 }
-              ** apply id in Hcont as Hcont'; revert Hcont Hcont'; rewrite {1}meet_left {1}meet_right; intros Hcont Hsim.
-               assert (local_steps O (<[i := (e_t', e_s)]> P)) as Hlocal.
-                 { eapply Hcont; [|done|].
-                   + eapply sim_expr_all_insert; first done.
-                     by rewrite sim_expr_unfold /sim_expr_body.
-                   + eapply list_lookup_insert, lookup_lt_Some, Hlook.
-                  }
-                 feed pose proof (Hlocal D').
-                 { rewrite list_fmap_insert //=. eapply active_exprs_update; auto. }
-                 { eapply local_all_weaken; first done. set_solver. }
-          ++ specialize (NoStutter _ _ Hstep) as (e_s' & T_s & Hstep_src & Hlen & Hsim).
-             exists (<[i := (e_t', e_s')]> P ++ zip T_f T_s), {[i]}.
-             rewrite !fmap_app fst_zip; last lia.
-             rewrite snd_zip; last lia.
-             rewrite !list_fmap_insert.
-             split; first done.
-             split.
-             { simpl. econstructor; [|eapply pool_no_steps|by rewrite left_id].
-               eapply pool_step_iff. exists e_s, e_s', T_s.
-               repeat split; eauto. by rewrite list_lookup_fmap Hlook. }
-             assert (local_steps (O ∖ {[i]}) (<[i := (e_t', e_s')]> P ++ zip T_f T_s)) as Hlocal.
-             { eapply IH; first by set_solver.
-               intros t s [Hin|Hin]%elem_of_app.
-               - eapply sim_expr_all_insert; [apply Hall| |apply Hin].
-                 eapply Hsim; simpl; set_solver.
-               - eapply Hsim; simpl; set_solver.
-             }
-             eapply Hlocal.
-             { rewrite fmap_app. etrans; first by eapply active_exprs_remove.
-               rewrite list_fmap_insert. eapply active_exprs_weaken. }
-        -- intros D P HD Hsub Hall Hlook.
-           rewrite /local_all lfp_fixpoint {1}/must_step.
-           intros Hdel.
-           right. split.
-           { destruct CanStep as (e' & T_f & Hstep).
-             exists (<[i := e']> P.*1 ++ T_f), i.
-             eapply pool_step_iff. do 3 eexists; split; first eauto.
-             split; last done. by rewrite list_lookup_fmap Hlook. }
-           intros T_t' D' j Hfair.
-           eapply fair_pool_step_inv in Hfair as (j_t & j_t' & T_f & Hstep & Hlook' & Hupd & HDj & Hdecr).
-           assert (i ≠ j) as Hij by congruence.
-           assert (∃ j_s, P !! j = Some (j_t, j_s)) as [j_s Hlook''].
-           { revert Hlook'. rewrite list_lookup_fmap.
-             destruct (P !! j) as [[]|]; simpl; naive_solver. }
-           clear Hlook'.
-           assert (sim_expr j_t j_s) as Hsim.
-           { eapply Hall, elem_of_list_lookup_2, Hlook''. }
-           eapply sim_expr_step in Hsim; last eauto.
-           destruct Hsim as [Stutter|NoStutter].
-           ++ exists (<[j := (j_t', j_s)]> P), ∅.
-              destruct Stutter as [-> Hsim].
-              rewrite !list_fmap_insert. subst T_t'.
-              split; first by rewrite right_id.
-              split.
-              { simpl; rewrite list_insert_id; eauto using pool_no_steps.
-                by rewrite list_lookup_fmap Hlook''. }
-              eapply Hdecr in HD as (x & Heq & HD'); last done.
-              assert (x = d) as -> by congruence; clear Heq.
-              eapply (local_all_weaken _ O); last set_solver.
-              eapply IHd; auto using sim_expr_all_insert; last first.
-              { rewrite list_lookup_insert_ne //. }
-              admit.
-              (* we have the same value distinction here as before,
-                 we should be able to remove the active_exprs assumption *)
-           ++ destruct NoStutter as (j_s' & T_s & Hsrc & Hlen & Hall').
-              exists (<[j := (j_t', j_s')]> P ++ zip T_f T_s), {[j]}.
-              (* analogous to the previous case:
-                 if j is still in O, then we have decreased O just now.
-                 if j is not in O, then the d has decreased for this O
-                 and we can use IHd. *)
-              admit.
-Admitted.
+  eapply gfp_greatest_post_fixpoint. rewrite /sim_pool_body.
+  enough (∀ O D P, sim_expr_all P → O ⊆ threads P.(tgt) → local_all P O D) by (intros ??; eauto).
+  induction O as [O IHO] using set_strong_ind.
+  intros D P Hall Hsub.
+  destruct (decide (O ≡ ∅)) as [Empty|[i Hel]%set_choose].
+  - rewrite lfp_fixpoint {1}/must_step. intros Hdel.
+    left. split; last done. intros i; set_solver.
+  - specialize (Hsub _ Hel) as Hthread.
+    eapply threads_spec in Hthread as (e & Hlook).
+    eapply list_lookup_fmap_inv in Hlook as ([e_t e_s] & -> & Hlook).
+    assert (sim_expr e_t e_s) as Hsim by eapply Hall, elem_of_list_lookup_2, Hlook.
+    revert Hsim; rewrite sim_expr_unfold /sim_expr_body; intros Hsim.
+    revert e_t e_s Hsim P Hall Hlook D Hsub.
+    change (lfp (sim_expr_inner sim_expr) ⪯
+            λ e_t e_s, ∀ P,
+              sim_expr_all P →
+              P !! i = Some (e_t, e_s) →
+              ∀ D, O ⊆ threads P.(tgt) → local_all P O D).
+    eapply lfp_strong_ind; first apply _.
+    intros e_t e_s Hinner P Hall Hlook D Hsub.
+    destruct Hinner as [Val|[CanStep AllSteps]].
+    + destruct Val as [Val_s Val_t].
+      eapply (local_all_add_values _ (O∖{[i]})).
+      * eapply IHO; auto; set_solver.
+      * intros j Hj; destruct (decide (i = j)); subst; last set_solver.
+        right; do 2 eexists; done.
+    + assert (¬ val e_t) as Hnval by naive_solver.
+      eapply local_all_delay_for; intros Hdom.
+      destruct (Hdom i) as [d HD]; last clear Hdom.
+      { apply active_threads_spec. eapply Hsub in Hel. eapply threads_spec in Hel.
+        destruct Hel as [e Hel]. exists e. revert Hel.
+        rewrite list_lookup_fmap Hlook //=. naive_solver.
+      }
+      revert D P HD Hsub Hall Hlook.
+      induction (lt_wf d) as [d _ IHd].
+      intros D P HD Hsub Hall Hlook.
+      rewrite lfp_fixpoint {1}/must_step; intros Hdel.
+      right. split.
+      { destruct CanStep as (e' & T_f & Hstep).
+        exists (<[i := e']> P.(tgt) ++ T_f), i.
+        eapply pool_step_iff. do 3 eexists; split; first eauto.
+        split; last done. by rewrite list_lookup_fmap Hlook. }
+      intros T_t' D' j Hpool.
+      eapply fair_pool_step_inv in Hpool as (e_j_t & e_j_t' & T_f  & Htgt & Hlookj & Hupd & Hdecr).
+      destruct (decide (i = j)).
+      * subst j. rewrite list_lookup_fmap Hlook //= in Hlookj.
+        assert (e_j_t = e_t) as -> by congruence; clear Hlookj.
+        rename e_j_t' into e_t'. destruct (AllSteps _ _ Htgt) as [[-> Steps]|NoStutter].
+        -- eapply local_all_stuttered; [by rewrite right_id in Hupd|done|].
+           eapply id in Steps as Steps'. (* FIXME: this step is not linear, but we should be able to make it linear *)
+           revert Steps Steps'; rewrite {1}meet_left meet_right.
+           intros IH Hsim.
+           change (lfp _ _ _) with (sim_expr_body sim_expr e_t' e_s) in Hsim.
+           revert Hsim; rewrite -sim_expr_unfold; intros Hsim.
+           eapply IH; eauto using sim_expr_all_insert, list_lookup_insert, lookup_lt_Some.
+           etrans; first eapply Hsub.
+           rewrite list_fmap_insert; eapply threads_update.
+        -- destruct NoStutter as (e_s' & T_s & Hsrc & Hlen & Hsims).
+           eapply local_all_not_stuttered; eauto.
+           eapply IHO; first set_solver; last first.
+           { rewrite fmap_app list_fmap_insert.
+            etrans; last eapply threads_weaken.
+            etrans; last eapply threads_update.
+            set_solver. }
+           eapply sim_expr_all_app; first eapply sim_expr_all_insert.
+           { done. }
+           { eapply Hsims; simpl; set_solver. }
+           { intros ???; eapply Hsims; simpl; set_solver. }
+        * eapply list_lookup_fmap_inv in Hlookj as ([e_j_t_ e_j_s] & -> & Hlookj).
+          rename e_j_t_ into e_j_t; simpl in Htgt.
+          assert (sim_expr e_j_t e_j_s) as Hsim by eapply Hall, elem_of_list_lookup_2, Hlookj.
+          eapply Hdecr in HD as (m & -> & HD'); last done.
+          eapply sim_expr_step in Hsim as [Stutter|NoStutter]; last done.
+          -- destruct Stutter as [-> Hsim].
+             eapply local_all_stuttered; [by rewrite right_id in Hupd|done|].
+             eapply IHd; eauto using sim_expr_all_insert.
+             { rewrite list_fmap_insert; by etrans; last eapply threads_update. }
+             { rewrite list_lookup_insert_ne //. }
+          -- destruct NoStutter as (e_j_s' & T_s & Hsrc & Hlen & Hsims).
+             eapply local_all_not_stuttered; eauto.
+             eapply (local_all_weaken _ O); last set_solver.
+             eapply IHd; eauto.
+             { rewrite fmap_app list_fmap_insert.
+               etrans; last eapply threads_weaken.
+               etrans; last eapply threads_update.
+               done. }
+            { eapply sim_expr_all_app; first eapply sim_expr_all_insert.
+              - done.
+              - eapply Hsims; simpl; set_solver.
+              - intros ???; eapply Hsims; simpl; set_solver. }
+            { eapply lookup_app_l_Some. by rewrite list_lookup_insert_ne. }
+Qed.
